C-verifier/src/Midend-IVL/Isabelle-UTP-Extended/examples/TotalCorrectness/Abrupt/examples_vcg_total.thy
@@ -72,7 +72,7 @@ lemma increment_tactic2:
 subsection \<open>Even count\<close>
 
 lemma even_count_tactic0:
-  assumes \<open>vwb_lens i\<close> and \<open>weak_lens start\<close> and \<open>vwb_lens j\<close> and \<open>weak_lens endd\<close>
+  assumes \<open>vwb_lens i\<close> and \<open>vwb_lens j\<close>
   and \<open>lens_indep_all [i, start, j, endd]\<close>
   shows
   \<open>\<lbrace>&start =\<^sub>u \<guillemotleft>0::int\<guillemotright> \<and> &endd =\<^sub>u 1\<rbrace>
@@ -106,7 +106,7 @@ lemma even_count_tactic0:
   oops
 
 lemma even_count_tactic1:
-  assumes \<open>vwb_lens i\<close> and \<open>weak_lens start\<close> and \<open>vwb_lens j\<close> and \<open>weak_lens endd\<close>
+  assumes \<open>vwb_lens i\<close> and \<open>vwb_lens j\<close>
   and \<open>lens_indep_all [i, start, j, endd]\<close>
   shows
   \<open>\<lbrace>&start =\<^sub>u \<guillemotleft>0::int\<guillemotright> \<and> &endd =\<^sub>u 1\<rbrace>
@@ -133,7 +133,7 @@ lemma even_count_tactic1:
   done
 
 lemma even_count_tactic2:
-  assumes \<open>vwb_lens i\<close> and \<open>weak_lens start\<close> and \<open>vwb_lens j\<close> and \<open>weak_lens endd\<close>
+  assumes \<open>vwb_lens i\<close> and \<open>vwb_lens j\<close>
   and \<open>i \<bowtie> start\<close> and \<open>i \<bowtie> j\<close>
   and \<open>lens_indep_all [i, start, j, endd]\<close>
   shows
